Update MachineTheory.v

MachineTheory.v
@@ -4,4 +4,42 @@ Import ListNotations.
 Import MACHINE.
 
 Section MachineTheory.
+Variables (m : Machine).
+
+(* State conservation law *)
+Definition act0 (f : state m → list (input m) → state m)
+:= ∀ s : state m, f s [] = s.
+(* Single impact law *)
+Definition act1 (f : state m → list (input m) → state m)
+:= ∀ (s : state m) (i : input m), f s [i] = pass m s i.
+(* Cumulative law *)
+Definition actC (f : state m → list (input m) → state m)
+:= ∀ (s : state m) (u' u'' : list (input m)),
+     f s (u' ++ u'') = f (f s u') u''.
+
+Lemma run0 : act0 (run m).
+Proof. unfold act0. trivial. Qed.
+
+Lemma run1 : act1 (run m).
+Proof. unfold act1. trivial. Qed.
+
+Lemma runC : actC (run m).
+Proof.
+  unfold actC. intros. revert s.
+  induction u' as [| i v IHu']; intro; simpl.
+  - reflexivity.
+  - exact (IHu' (pass m s i)).
+Qed.
+
+Theorem run_uniqueness : ∀ (f : state m → list (input m) → state m),
+  act0 f → act1 f → actC f 
+    → ∀ (s : state m) (u : list (input m)), f s u = run m s u.
+Proof.
+  intros * H0 H1 HC *. revert s.
+  induction u as [| i u' IHu]; intro; simpl.
+  - apply H0.
+  - assert (H : [i] ++ u' = i :: u'). { trivial. }
+    rewrite <- H. rewrite (HC s [i] u').
+    rewrite <- (H1 s). apply IHu.
+Qed.
 End MachineTheory.
